---
title: Discrete-time Signal Processing (1)
date: 2024-10-23 19:50:38
tags: ['Study','Signal Processing']
categories: Notes
index_img:
cover:
description: Notes about Fourier Transform
---

# Discrete-Time Signals

## Define
A discrete-time signal is a sequence of numbers that are defined at discrete points in time. It is often represented as a function of an integer variable, such as $x[n]$ or $x(n)$, where $n$ is the time index.

$$x={x[n]},n \in Z$$

This sequence can be sampled from a continuous-time signal $x(t)$

$$x[n] = x_a(nT), ,n \in Z$$

where T is the sampling period and its $\frac{1}{T}$ is the sampling frequency.

## Basic sequences

### Unit sample  

$$\delta[n]=\left\{\begin{matrix} 1, & n=0\\  0, & n\neq 0 \end{matrix}\right.$$

![](https://cdn.jsdelivr.net/gh/AtomChen0425/picx-images-hosting@master/Evolution-Algorithms/image.8ojp1mp0nq.webp)

Any sequence can be expressed as

$$x[n] = \displaystyle{ \sum_{k=-\infty}^{\infty}x[k]\delta[n-k] }$$


### Unit step

$$u[n]=\left\{\begin{matrix} 1, & n\geq 0\\  0, & n< 0 \end{matrix}\right.$$

![](https://cdn.jsdelivr.net/gh/AtomChen0425/picx-images-hosting@master/Signal-process/image.4qrbkyg61b.webp)

It also can be expressed as

$$u[n] = \displaystyle{ \sum_{k=-\infty}^{n}\delta[k] }$$

$$u[n] = \displaystyle{ \sum_{k=0}^{\infty}\delta[n-k] }$$

$$\delta[n] = u[n] - u[n-1]$$
### Exponential

![](https://cdn.jsdelivr.net/gh/AtomChen0425/picx-images-hosting@master/Signal-process/image.4uaxipwut4.webp)

$$x[n] = Aa^n u[n]$$

If A,Î± are both complex numbers

$$\left\{\begin{matrix} A& = & |A|(cos\phi+jsin\phi)&=&|A|e^{j\phi} \\  \alpha & = & |\alpha|(cos\omega_0+jsin\omega_0) &=&|\alpha|e^{j\omega_0} \end{matrix}\right.$$

Then 

$$\begin{align*} x[n] &= A\alpha^n\\   &= |A|e^{j\phi}|\alpha|^ne^{j\omega_0n}\\   &= |A||\alpha|^ne^{j(\omega_0n+\phi)}\\  &= |A||\alpha|^ncos(\omega_0n+\phi)+j|A||\alpha|^nsin(\omega_0n+\phi) \end{align*}$$

When $\alpha=1$

$$x[n] = |A|e^{j(\omega_0n+\phi)} = |A|cos(\omega_0n+\phi)+j|A|sin(\omega_0n+\phi)$$
### Sinusoid

![](https://cdn.jsdelivr.net/gh/AtomChen0425/picx-images-hosting@master/Signal-process/image.361klj70vt.webp)

$$x[n] = A\sin(\omega_0n+\phi)$$

## Difference between discrete-time sinusoidal series and continuous-time sinusoidal signals

### Frequency

Assuming a frequency $(\omega_0 + 2\pi)$

If it is a continuous time sinusoidal signal, then there are

$$f(t) = Acos((\omega_0+2\pi)t + \phi)$$

If it is a discrete-time sinusoidal signal, then there are

$$x[n] = Acos[\omega_0n+2\pi n + \phi] = Acos[\omega_0 n + \phi]$$

We can see that discrete-time sinusoidal sequences with frequency $(\omega_0 + 2\pi k)$ (where k is an arbitrary integer) are indistinguishable from each other, i.e., the frequency remains $\omega_0$

### Period

For continuous time sinusoidal signals

$$f(t) = Acos(\omega_0t+\phi)$$
The period of this signal $T=\frac{2\pi}{\omega_0}$

For discrete-time sinusoidal signals

$$x[n] = Acos[\omega_0n+\phi]$$

In the discrete time case, a periodic sequence should satisfy

$$x[n] = x[n+N]$$

The period N in Equation must be an integer. If this condition is used to test the periodicity of a discrete-time sinusoidal sequence, we have

$$Acos(\omega_0n+\phi) = Acos(\omega_0n+\omega_0N+\phi)$$


$$\omega_0N = 2\pi k$$

Where k is an integer. It can be seen that the value of the period N is not necessarily equal to $\frac{2\pi}{\omega_0}$, this is because N must be an integer.

# Discrete-time systems

Mathematically defined as transformation that maps input sequence x[n] into an output y[n]

![](https://cdn.jsdelivr.net/gh/AtomChen0425/picx-images-hosting@master/Signal-process/image.1vynf85qyb.webp)

## Memoryless System

If the output y[n] at every value of n depends only on the input x[n] at the same value of n.

Exp.
$$y[n] = (x[n])^2 , for\space each\space n$$

## Linear Systems

Defined by the principle of superposition for its input and output.

It satisfies the following two conditions:

$$\begin{align*} &T\{x_1[n]+x_2[n]\} &=& T\{x_1[n]\}+T\{x_2[n]\} &=& y_1[n]+y_2[n]\\ &T\{ax[n]\}&=&aT\{x[n]\}&=&ay[n] \end{align*}$$

Where  `a` is an arbitrary constant. The combination of these two properties is known as the principle of superposition and is written as 

$$T\{ax_1[n]+bx_2[n]\} = aT\{x_1[n]\}+bT\{x_2[n]\}$$

**Example:**

![](https://cdn.jsdelivr.net/gh/AtomChen0425/picx-images-hosting@master/Signal-process/image.2veqseu8du.webp)

## Time-Invariant Systems

A system for which a time shift or delay of the input sequence causes a corresponding shift in the output sequence.
$$T\{x[n-n_0]\} = y[n-n_0]$$

![](https://cdn.jsdelivr.net/gh/AtomChen0425/picx-images-hosting@master/Signal-process/image.3d4sgzwfci.webp)

## Causal Systems

When the output at sample n, i.e. y[n], only depends on the present and/or past values of input x[n]. The value of the output sequence at n = n0 depends only on the value of the input sequence at n <= n0

![](https://cdn.jsdelivr.net/gh/AtomChen0425/picx-images-hosting@master/Signal-process/image.1ovfjt6ixy.webp)

## Stability

(in BIBO sense) A system where the response of finite inputs do not diverge.

$$|x[n]|\leqslant B_x < \infty,\ for\ each\ n$$
$$|y[n]|\leqslant B_y < \infty,\ for\ each\ n$$

![](https://cdn.jsdelivr.net/gh/AtomChen0425/picx-images-hosting@master/Signal-process/image.5j472rpang.webp)

# LTI Systems

These systems are both Linear and Time Invariant.

They have significant applications in DT signal processing.

There is a very convenient representation form for these systems, using convolutional sum.

$$y[n] = x[n]*h[n] = \sum_{k=-\infty}^{\infty}x[k]h[n-k]$$

Where `*` denotes convolution operation.

Where `h[n]` is called the impulse response of the system.

**Important Formula**

$$\sum_{k=N1}^{N2}a^k = \frac{a^{N_1} - a^{N_2+1}}{1-a}$$

## Properties of LTI Systems

### Commutative property:

$$\begin{align*} y[n] &=x[n]*h[n] \\  &=\sum_{m=-\infty}^{\infty}x[n-m]h[m]  \\   &=\sum_{p=-\infty}^{\infty}x[p]h[n-p] \quad letting\ p=n-m \\   &=\sum_{p=-\infty}^{\infty}h[n-p]x[p] \\  &=h[n]*x[n]  \end{align*}$$

![](https://cdn.jsdelivr.net/gh/AtomChen0425/picx-images-hosting@master/Signal-process/image.7p3lok5i59.webp)

### Associative property:

$$\begin{align*} y[n] &=(x[n]*h_1[n])*h_2[n] \\  &=z[n]*h_2[n] \\  &=\sum_{m=-\infty}^{\infty}z[n-m]h_2[m] \\  &=\sum_{p=-\infty}^{\infty}z[p]h_2[n-p] \quad letting\ p=n-m\\   &=\sum_{p=-\infty}^{\infty}\left ( \sum_{i=-\infty}^{\infty}x[p-i]h_1[i] \right )h_2[n-p] \\   &=\sum_{p=-\infty}^{\infty}\left ( \sum_{q=-\infty}^{\infty}x[q]h_1[p-q] \right )h_2[n-p] \quad letting\ q=p-i\\  &=\sum_{q=-\infty}^{\infty}x[q]\left ( \sum_{p=-\infty}^{\infty}h_1[p-q]h_2[n-p] \right ) \\  &=\sum_{q=-\infty}^{\infty}x[q]\left ( \sum_{m=-\infty}^{\infty}h_1[n-q-m]h_2[m] \right ) \\  &=\sum_{k=-\infty}^{\infty}x[n-k]\left ( \sum_{m=-\infty}^{\infty}h_1[k-m]h_2[m] \right ) \quad letting\ k=n-q \\  &=x[n]*(h_1[n]*h_2[n]) \end{align*}$$

![](https://cdn.jsdelivr.net/gh/AtomChen0425/picx-images-hosting@master/Signal-process/image.7ax5xoxluk.webp)

### Distributive property:

$$\begin{align*} y[n] &=x[n]*h[n] \\  &=x[n]*(h_1[n]+h_2[n]) \\  &=\sum_{m=-\infty}^{\infty}x[n-m](h_1[m]+h_2[m])  \\   &=\sum_{m=-\infty}^{\infty}x[n-m]h_1[m]+\sum_{m=-\infty}^{\infty}x[n-m]h_2[m] \\   &=x[n]*h_1[n]+x[n]*h_2[n]  \end{align*}$$

![](https://cdn.jsdelivr.net/gh/AtomChen0425/picx-images-hosting@master/Signal-process/image.41y211aeuw.webp)

### Time shifting property:

If $ð‘¦[ð‘›] = ð‘¥[ð‘›] âˆ— â„Ž[ð‘›]$ , then
$ð‘¥[ð‘› âˆ’ ð‘›1] âˆ— â„Ž [ð‘› âˆ’ ð‘›2] = ð‘¦ [ð‘› âˆ’ ð‘›1 âˆ’ ð‘›2]$

### Causallity:
An LTI system is causal if and only if  $â„Ž[ð‘›] = 0$ for $ð‘› < 0$ , then $ð‘¦[ð‘›] = 0$ for $ð‘› < 0$

### Finite
If ð‘¥[ð‘›] and â„Ž[ð‘›] are of finite duration, then ð‘¦[ð‘›] is of finite duration.

In particular, if ð‘¥[ð‘›] is of length ð‘1, and â„Ž[ð‘›] is of length ð‘2, then ð‘¦[ð‘›] is of length ð‘1 +ð‘2 âˆ’1.

### Stability:
An LTI system is BIBO stable if and only if 
$$\sum_{k=-\infin}^{\infin}|â„Ž[k]| < \infin$$ 

## EXAMPLE
### Delay system

$$y[n] = x[n-n_d]$$

$$h[n] = \delta[n-n_d]$$

### Moving averag

$$y[n] = \frac{1}{M_1+M_2+1}\displaystyle{ \sum_{k=-M_1}^{M_2}x[n-k] }$$

$$\begin{align*} h[n] &=\frac{1}{M_1+M_2+1}\sum_{k=-M_1}^{M_2}\delta[n-k] \\ &=\left \{\begin{matrix} \frac{1}{M_1+M_2+1}, & -M_1\leqslant n\leqslant M_2 \\  0, & \ else  \end{matrix}\right.\\ &=\frac{1}{M_1+M_2+1}(u[n+M_1]-u[n-M_2-1]) \\ &=\frac{1}{M_1+M_2+1}(\delta[n+M_1]-\delta[n-M_2-1])*u[n] \end{align*}$$

### Accumulator

$$y[n] = \displaystyle{ \sum_{k=-\infty}^{n}x[k] }$$

$$\begin{align*} h[n] &= \sum_{k=-\infty}^{n}\delta[k]\\   &=\sum_{k=-\infty}^{0}\delta[n+k] \\   &= \left\{\begin{matrix} 1 &,n\geqslant 0 \\  0 &,n<0  \end{matrix}\right. \\ &=u[n] \end{align*}$$

### Forward difference

$$y[n] = x[n+1]-x[n]$$

$$h[n] = \delta[n+1]-\delta[n]$$

### Backward difference

$$y[n] = x[n]-x[n-1]$$

$$h[n] = \delta[n]-\delta[n-1]$$

# Linear Constant-Coefficient Difference Equations

They are an important class of LTI systems where the input x[n] and the output y[n] satisfy an Nth order linear constant coefficient difference equation as follows:

$$\displaystyle{ \sum_{k=0}^{N}a_k y[n-k]=\sum_{m=0}^{M}b_m x[n-m] }$$

When we solve the difference equation, we will assume $y_h[n] = Az^n$

Then we can get 

$$\displaystyle{ \sum_{k=0}^{N}a_k z^{-k} } = 0$$
$$y_h[n] = \displaystyle{ \sum_{m=1}^{N}A_m z_m^n }$$

## initial-rest condition

$$if\ x[n]=0,\  n<n_0 \quad then \ y[n]=0,\  n<n_0 $$

# Frequency domain representation of signals and systems

For an LTI system, if the input is $x[n] = e^{j\omega n},-\infty<n<\infty$
then the output is

$$\begin{align*} y[n] &=  \sum_{k=-\infty}^{\infty}h[k]x[n-k] \\ &=\sum_{k=-\infty}^{\infty}h[k]e^{j\omega(n-k)}\\ &=\sum_{k=-\infty}^{\infty}h[k]e^{-j\omega k}e^{j\omega n} \end{align*}$$

$$H(e^{j\omega}) = \displaystyle{ \sum_{k=-\infty}^{\infty}h[k]e^{-j\omega k} }$$

It can be observed that eigenvalues $H(e^{j\omega})$ are a function Ï‰ of frequency dependent, so eigenvalues $H(e^{j\omega})$ are also known as the frequency response of the system. Generally, $H(e^{j\omega})$ it is a complex number and can be divided into real and imaginary representations

$$H(e^{j\omega}) = H_R(e^{j\omega}) + jH_I(e^{j\omega})$$

$$H(e^{j\omega}) = |H(e^{j\omega})|e^{j\angle H(e^{j\omega)}}$$

And the Frequency response has periodicity.

$$\begin{align*} H(e^{j(\omega+2\pi)}) &= \sum_{n=-\infty}^{\infty}h[n]e^{-j(\omega+2\pi)n} \\ &= \sum_{n=-\infty}^{\infty}h[n](e^{-j\omega n}e^{-j2\pi n})\\ &= \sum_{n=-\infty}^{\infty}h[n]e^{-j\omega n}\\ &= H(e^{j\omega}) \end{align*}$$


If

$$x[n] = Acos (\omega_0 + \phi) = \frac{A}{2}e^{j\phi}e^{j\omega_0 n} + \frac{A}{2}e^{-j\phi}e^{-j\omega_0 n}$$

Then

$$\begin{align*} y[n] &= \frac{A}{2}\{H(e^{j\omega_0})e^{j\theta}e^{j\omega_0 n}+H(e^{-j\omega_0})e^{-j\theta}e^{-j\omega_0 n} \} \\ &= \frac{A}{2}\{[H_R(e^{j \omega_0})+jH_I(e^{j\omega_0})]e^{j\theta}e^{j\omega_0 n}+[H_R(e^{j \omega_0})-jH_I(e^{j\omega_0})]e^{-j\theta}e^{-j\omega_0 n} \} \\ &\qquad h[n]\ is\ real\Rightarrow H(e^{-j\omega_0})=H^{*}(e^{j\omega_0})\\ &= \frac{A}{2}\{ H_R(e^{j\omega_0})(e^{j\theta}e^{j\omega_0 n}+e^{-j\theta}e^{-j\omega_0 n})+jH_I(e^{j\omega_0})(e^{j\theta}e^{j\omega_0 n}-e^{-j\theta}e^{-j\omega_0 n}) \} \\ &= \frac{A}{2} \{ 2H_R(e^{j\omega_0})cos(\omega_0 n + \theta) - 2H_I(e^{j\omega_0})sin(\omega_0 n + \theta) \} \\ &= A \{ H_R(e^{j\omega_0})cos(\omega_0 n + \theta) - H_I(e^{j\omega_0})sin(\omega_0 n + \theta) \} \\ &= A\{ |H(e^{j\omega_0})|cos(\phi)cos(\omega_0 n +\theta)-|H(e^{j\omega_0})|sin(\phi)sin(\omega_0 n +\theta)\} \quad letting\ \phi=\angle H(e^{j\omega_0})\\ &= A |H(e^{j\omega_0})| cos(\omega_0 n +\theta+\phi) \end{align*}$$

# Discrete-Time Fourier Transform

$${X(e^{j\omega}) = \displaystyle{ \sum_{n=-\infty}^{\infty}x[n]e^{-j\omega n} }}$$

$${\displaystyle{x[n] = \frac{1}{2\pi}\int_{-\pi}^{\pi}X(e^{j\omega})e^{j\omega n}d\omega }}$$

$$x[n] = x_e[n]+x_o[n]$$

$$\left\{\begin{matrix} x_e[n] &=&\frac{1}{2}(x[n]+x^*[-n]) &=&x_e^*[-n] \\  x_o[n] &=&\frac{1}{2}(x[n]-x^*[-n]) &=&-x_o^*[-n]  \end{matrix}\right.$$

$$X(e^{j\omega}) = X_e(e^{j\omega})+X_o(e^{j\omega})$$

$$\left\{\begin{matrix} X_e(e^{j\omega}) &=&\frac{1}{2}[X(e^{j\omega})+X^*(e^{j\omega})] &=&X_e^*(e^{j\omega}) \\  X_o(e^{j\omega}) &=&\frac{1}{2}[X(e^{j\omega})-X^*(e^{j\omega})] &=&-X_o^*(e^{j\omega})  \end{matrix}\right.$$

![](https://cdn.jsdelivr.net/gh/AtomChen0425/picx-images-hosting@master/Signal-process/image.8z6iwc87fz.webp)

![](https://cdn.jsdelivr.net/gh/AtomChen0425/picx-images-hosting@master/Signal-process/image.pfc84ewye.webp)

![](https://cdn.jsdelivr.net/gh/AtomChen0425/picx-images-hosting@master/Signal-process/image.2rv4w6dy3t.webp)


